Start fixing dumb failure in models

TransVal/smt.v
@@ -13,11 +13,28 @@ evalSexp evaluates an SMT expression given an environment that must! be total on
 every variable that may occur in a formula.
 **)
 
-Definition evalSexp E s : val(*bitvec*) :=
-match exp_eval E s with
-|Some v => v
-|None => default_val
-end.
+Definition to_partial (E:env val) x : option val (*bitvec*) := Some (E x).
+Definition to_total (E:onv val) x : val :=
+  match E x with
+    |Some v => v
+    |None => default_val
+  end.
+
+Lemma agree_on_partial lv E E'
+: agree_on eq lv E E'
+  -> agree_on eq lv (to_partial E) (to_partial E').
+Proof.
+  intros; unfold to_partial; hnf; intros; simpl.
+  rewrite H; eauto.
+Qed.
+
+Lemma agree_on_total lv E E'
+: agree_on eq lv E E'
+  -> agree_on eq lv (to_total E) (to_total E').
+Proof.
+  intros; unfold to_total; hnf; intros; simpl.
+  rewrite H; eauto.
+Qed.
 
 (** Define what uninterpreted function symbols are **)
 Definition pred := lab (*arglst -> bool*).
@@ -31,9 +48,9 @@ Inductive smt :Type :=
 | smtImp: smt -> smt -> smt
 | constr: exp -> exp -> smt
 | funcApp: pred -> arglst -> smt
-|smtReturn:  exp -> smt
-|smtFalse: smt
-|smtTrue:smt.
+| smtReturn:  exp -> smt
+| smtFalse: smt
+| smtTrue:smt.
 
 (** Now define the parameters for the translation function **)
 Inductive pol:Type :=
@@ -46,22 +63,9 @@ match el with
 |_:: el' => default_val :: listGen el'
 end.
 
-Definition evalList E (e:arglst) : vallst :=
-match (omap (exp_eval E) e) with
-|Some el => el
-| None => listGen e
-end.
-(*match e with
-|nil =>  nil
-|x::e' => (evalSexp E x) :: ( evalList E e')
-end.*)
-
-Definition evalSpred (F :pred->  vallst -> bool) (f:lab) (e:vallst)  :=
-F f e.
-
 (** models relation for smt. No need for options here too, because if models can be evaluated by an environment,
 every variable must have been defined. **)
-Fixpoint models (F:pred ->vallst->bool) E (s:smt) : Prop:=
+Fixpoint models (F:pred ->vallst->bool) (E:env val) (s:smt) : Prop:=
 match s with
   |smtAnd a b
    => (models F E a) /\ (models F E b)
@@ -70,23 +74,27 @@ match s with
   |smtNeg a
    =>  (models F E a) -> False
 | ite c t f
-  => match evalSexp E c with
-       |  v
-         => if val2bool v
+  => match exp_eval (to_partial E) c with
+       |  Some v
+          => if val2bool v
             then models F E t
             else models F E f
+       | _ => False
      end
 |smtImp a b
  => (models F E a) ->(models F E b)
-|constr s1 s2 => match evalSexp E s1,  evalSexp E s2 with
-                   |b1, b2 => val2bool( bvEq b1 b2)
+|constr s1 s2 => match exp_eval (to_partial E) s1,  exp_eval (to_partial E) s2 with
+                  |Some b1, Some b2 => val2bool( bvEq b1 b2)
+                  | _, _ => False
                  end
-|funcApp f a => match evalList E a with
-                  | l  => evalSpred F (labInc f 1) l
+|funcApp f a => match omap (exp_eval (to_partial E)) a with
+                  | Some l  => F (labInc f 1) l
+                  | None => False
                 end
 |smtReturn e
- => match evalSexp E e with
-        |  v => evalSpred F (LabI 0) (v::nil)
+ => match exp_eval (to_partial E) e with
+     | Some v => F (LabI 0) (v::nil)
+     | _ => False
     end
 |smtFalse => False
 |smtTrue => True
