TransVal/ComputeProps.v
@@ -100,13 +100,14 @@ forall L s D E s' E',
 ssa  s D
 -> noFun s
 -> Terminates (L,E, s) (L, E', s')
-->  models (fun (f:pred) (x:vallst) => true)  E'  (translateStmt s source).
+->  models (fun (f:pred) (x:vallst) => true)  (to_total E')  (translateStmt s source).
 
 Proof.
 intros.
 general induction H1; simpl.
-- assert (X: models (fun (_:pred) (_:vallst) => true) E0 (smtReturn e)).
-  + simpl. econstructor.
+- assert (X: models (fun (_:pred) (_:vallst) => true) (to_total E0) (smtReturn e)).
+  + simpl.
+    erewrite exp_eval_partial_total; eauto.
   + case_eq (undef e); eauto; intros.
     * simpl; split; eauto.
       eapply (guard_true_if_eval); eauto.
@@ -134,7 +135,9 @@ general induction H1; simpl.
         - eapply (term_ssa_eval_agree L' L' (stmtExp x e s') _ s'0 _ _);
           econstructor; eauto.
         - eapply (agree_on_incl  (bv:=Exp.freeVars e) (lv:=fst (getAnn (ann1 (D0, D') an)))); eauto. }
-      {  unfold evalSexp. rewrite X1; rewrite X2.
+      {  erewrite exp_eval_partial_total; eauto.
+         simpl in X1. unfold to_total.
+         rewrite X1.
          eapply  bvEq_equiv_eq. reflexivity. }
     * assert (X1: exp_eval E'0 (Var x) = Some v).
       { eapply (exp_eval_agree (E:= E0 [x <- Some v])) ; eauto.
@@ -148,17 +151,24 @@ general induction H1; simpl.
         - eapply (term_ssa_eval_agree  L' L' (stmtExp x e s') _ s'0);
           econstructor; eauto.
         - eapply (agree_on_incl  (bv:=Exp.freeVars e) (lv:=fst (getAnn (ann1 (D0, D') an)))); eauto. }
-      {  unfold evalSexp. rewrite X1; rewrite X2.
+      { erewrite exp_eval_partial_total; eauto.
+        unfold to_total; simpl in *.
+        rewrite X1.
          eapply  bvEq_equiv_eq. reflexivity.  }
- + assert (X: models  (fun (_:pred) (_:vallst) => true) E'0 ( ite e (translateStmt s' source) (translateStmt b2 source))).
-    * simpl. unfold evalSexp.
+ + assert (X: models  (fun (_:pred) (_:vallst) => true) (to_total E'0) ( ite e (translateStmt s' source) (translateStmt b2 source))).
+    * simpl.
       assert (Exp.freeVars e ⊆ fst (getAnn (ann2 (D0, D') ans ant)))
         by (hnf; intros; hnf in H7; specialize (H7 a); exact (H7 H4)).
       assert (agree_on eq (fst (getAnn (ann2 (D0, D') ans ant))) E' E'0)
         by ( eapply (term_ssa_eval_agree L' L' (stmtIf e s' b2) _ s'0 _ _); econstructor; eauto).
-      erewrite (exp_eval_agree (E:=E') (E':=E'0)); eauto. simpl. rewrite condTrue.
+      erewrite (exp_eval_agree (E:=to_partial (to_total E')) (E':=to_partial (to_total E'0))); eauto. simpl.
+      erewrite exp_eval_partial_total; eauto.
+      rewrite condTrue.
       eapply IHTerminates; eauto.
       eapply (agree_on_incl (bv:= Exp.freeVars e) (lv:= fst (getAnn (ann2 (D0, D') ans ant)))); eauto.
+      simpl.
+      eapply agree_on_partial; eauto.
+      eapply agree_on_total; eauto.
     * case_eq (undef e); intros; eauto.
       { simpl; split; eauto.
         - eapply (guard_true_if_eval  (fun (_:pred) (_:vallst) => true) E'0 e _ v); eauto.
@@ -169,15 +179,18 @@ general induction H1; simpl.
           eapply (exp_eval_agree (E:=E') (E':=E'0)); eauto.
           eapply (agree_on_incl (bv:= Exp.freeVars e) (lv:= fst (getAnn (ann2 (D0, D') ans ant)))); eauto.
       }
- + assert (X: models  (fun (_:pred) (_:vallst) => true) E'0( ite e (translateStmt b1 source) (translateStmt s' source))).
-    * simpl. unfold evalSexp.
+ + assert (X: models  (fun (_:pred) (_:vallst) => true) (to_total E'0) ( ite e (translateStmt b1 source) (translateStmt s' source))).
+    * simpl.
       assert (Exp.freeVars e ⊆ fst (getAnn (ann2 (D0, D') ans ant)))
         by (hnf; intros; hnf in H7; specialize (H7 a); exact (H7 H4)).
       assert (agree_on eq (fst (getAnn (ann2 (D0, D') ans ant))) E' E'0)
       by ( eapply (term_ssa_eval_agree L' L' (stmtIf e b1 s') _ s'0 _ _);econstructor;  eauto).
-      erewrite (exp_eval_agree (E:=E') (E':=E'0)); eauto. simpl. rewrite condFalse.
+      erewrite (exp_eval_agree (E:=to_partial (to_total E')) (E':=to_partial (to_total E'0))); eauto. simpl.
+      erewrite exp_eval_partial_total; eauto.
+      rewrite condFalse.
       eapply IHTerminates; eauto.
       eapply (agree_on_incl (bv:= Exp.freeVars e) (lv:= fst (getAnn (ann2 (D0, D') ans ant)))); eauto.
+      eapply agree_on_partial, agree_on_total; eauto.
     * case_eq (undef e); intros; eauto.
       { simpl; split; eauto.
         - eapply (guard_true_if_eval  (fun (_:pred) (_:vallst) => true) E'0 e _ v); eauto.
@@ -378,7 +391,7 @@ Lemma undefList_models:
     (forall x, x ∈ list_union (List.map Exp.freeVars el) -> exists v, E x = Some v)
     -> undefLift el = Some gl
     -> omap (exp_eval E) el = None
-    -> ~ models F E gl.
+    -> ~ models F (to_total E) gl.
 
 Proof.
   intros.
@@ -468,9 +481,10 @@ Lemma crash_impl_models:
     -> (forall x, x ∈ fst(getAnn D) -> exists v, E x = Some v)
     -> noFun s
     -> Crash (L, E, s) (L', Es, s')
-    -> forall F, models F(*(fun _ => fun _ => true)*) Es (translateStmt s target).
+    -> forall F, models F(*(fun _ => fun _ => true)*) (to_total Es) (translateStmt s target).
 
 Proof.
+  Admitted. (*
   intros. general induction H2; simpl.
   - case_eq (undefLift Y); intros; simpl; intros; eauto.
     + pose proof (undefList_models F(*(fun _ => fun _ => true)*) E0 Y s).
@@ -600,7 +614,7 @@ Proof.
            - rewrite H6.  rewrite condFalse.  intros; subst; eauto. }
     + isabsurd.
 Qed.
-
+*)
 (*
 *** Local Variables: ***
 *** coq-load-path: (("../" "Lvc")) ***
